PLT.v
@@ -1,0 +1,69 @@
+Require Import Coq.Lists.List.
+
+Import ListNotations.
+
+Definition var := nat.
+
+Section Syntax.
+
+Class Primitive (PL: Set) := {
+  prim: PL -> Prop
+}.
+
+Class Skip (PL: Set) := {
+  skip: PL
+}.
+
+Class Comp (PL: Set) := {
+  comp: PL -> PL -> PL
+}.
+
+Class Branching (PL: Set) (TL: Set) := {
+  ite: TL -> PL -> PL -> PL
+}.
+
+Class Looping (PL: Set) (TL: Set) := {
+  while: TL -> PL -> PL
+}.
+
+Class Imperative (PL: Set) (TL: Set)
+    {the_prim: Primitive PL}
+    {the_skip: Skip PL} {the_comp: Comp PL}
+    {the_ite: Branching PL TL} {the_while: Looping PL TL} := {
+  access: PL -> list var
+; change: PL -> list var
+; depends: TL -> list var
+; access_skip: access skip = []
+; change_skip: change skip = []
+; access_comp S1 S2: access (comp S1 S2) = access S1 ++ access S2
+; change_comp S1 S2: change (comp S1 S2) = change S1 ++ change S2
+; access_ite B S1 S2: access (ite B S1 S2) = depends B ++ access S1 ++ access S2
+; change_ite B S1 S2: change (ite B S1 S2) = change S1 ++ change S2
+; access_while B S1: access (while B S1) = depends B ++ access S1
+; change_while B S1: change (while B S1) = change S1
+}.
+
+Class Choice (PL: Set) := {
+  choice: PL -> PL -> PL
+}.
+
+Class Parallel (PL: Set) := {
+  par: PL -> PL -> PL
+}.
+
+Class Assert (PL: Set) (TL: Set) := {
+  assert: TL -> PL
+}.
+
+Class Micro (PL: Set) (TL: Set) `{Imperative PL TL}
+    {the_choice: Choice PL} {the_par: Parallel PL}
+    {the_assert: Assert PL TL} := {
+  access_choice S1 S2: access (choice S1 S2) = access S1 ++ access S2
+; change_choice S1 S2: change (choice S1 S2) = change S1 ++ change S2
+; access_par S1 S2: access (par S1 S2) = access S1 ++ access S2
+; change_par S1 S2: change (par S1 S2) = change S1 ++ change S2
+; access_assert B: access (assert B) = depends B
+; change_assert B: change (assert B) = []
+}.
+
+End Syntax.
